\documentclass[bigger]{beamer}

\input{header-beam} % change to header-handout for handouts

% ====================
\title[Lecture 9]{Logic I F13 Lecture 9}
\date{October 8, 2013}
% ====================

\include{header}


\setlength{\fitchprfwidth}{5em}

\section{Proof Strategies}

\subsec{Strategy for Proving Conjunctions}{

\begin{tabular}{@{}lp{13em}}
\fitchprf{
   \pline[1.]{}
}{
 \ellipsesline \\
 \pline[2.]{} \\
 \ellipsesline \\
 \pline[3.]{} \\
 \pline[4.]{P \land Q}[\hphantom{\landi{2, 3}}]
} 
  &
If we want to prove $\sf P \land Q$, we have to use $\land$Intro.
\end{tabular}

}

\subsec{Strategy for Proving Conjunctions}{

\begin{tabular}{@{}lp{13em}}
  \fitchprf{\pline[1.]{}}{
    \ellipsesline \\
    \pline[2.]{P} \\
    \ellipsesline \\
    \pline[3.]{Q} \\
    \pline[4.]{P \land Q}[\landi{2, 3}]
  } 
  &
  For $\land$Intro, we need to prove $\sf P$ first, then prove $\sf Q$. For the last line,
  we'll cite the lines where we proved $\sf P$ and  $\sf Q$, and use $\land$Intro.
\end{tabular}
}



\subsec{Strategy for Using Conjunctions}{

\begin{tabular}{@{}lp{13em}}
\fitchprf{
   \pline[1.]{P \land Q}
}{
 \pline{}[\hphantom{\lande{1}}] \\
 \pline{} \\
 \ellipsesline \\
 \pline{R}
} 
  &
If we want to use a sentence of the form $\sf P \land Q$ which is one
of our premises, or a sentence we've already proved, use $\land$Elim.
\end{tabular}
}

\subsec{Strategy for Using Conjunctions}{

\begin{tabular}{@{}lp{13em}}
\fitchprf{
   \pline[1.]{P \land Q}
}{
 \pline[2.]{P}[\lande{1}]\\
 \pline[3.]{Q}[\lande{1}]\\
 \ellipsesline \\
 \pline{R}
} 
& Use $\land$Elim to ``split up'' $\sf P \land Q$, proving both $\sf
P$ and $\sf Q$.  We'll probably need them further down in the proof.
\end{tabular}
}


\subsec{Strategy for Proving Disjunctions}{

\begin{tabular}{@{}lp{13em}}
\fitchprf{
   \pline[1.]{}
}{
 \ellipsesline \\
 \pline[2.]{} \\
 \pline[3.]{P \lor Q}[\hphantom{\lori{2}}]
} 
  &
We want to prove $\sf P \lor Q$. We could do this using  $\lor$Intro.
\end{tabular}
}


\subsec{Strategy for Proving Disjunctions}{

\begin{tabular}{@{}lp{13em}}
\fitchprf{\pline[1.]{}}{
\ellipsesline \\
\pline[2.]{P} \\
\pline[3.]{P \lor Q}[\lori{2}]
} 
&
For $\lor$Intro, we need to prove one of the disjuncts.
We'll try $\sf P$ first. For the last line,
we'll cite the line where we proved $\sf P$, and use $\lor$Intro.
\end{tabular}
}

\subsec{Strategy for Proving Disjunctions}{

\begin{tabular}{@{}lp{13em}}
\fitchprf{\pline[1.]{}}{
\ellipsesline \\
\pline[2.]{Q} \\
\pline[3.]{P \lor Q}[\lori{2}]
} 
&
If we can't prove $\sf P$, we may have to backtrack and try to prove $\sf Q$
instead.  Again, we'll cite the line where we proved $\sf Q$, and use
$\lor$Intro.
\end{tabular}
}


\subsec{Strategy for Using Disjunctions}{

\begin{tabular}{@{}l@{}p{13em}}
\fitchprf{
   \pline[1.]{P \lor Q}
}{
 \pline{}\\
\pline{} \\
\pline{}\\
\pline{} \\
\pline{} \\
\pline{} \\
\ellipsesline \\[.7em]
  \pline[6.]{R}[\hphantom{\lore{1}{2--3}{4--5}}]
} 
  &
Suppose we want to prove R, and we have $\sf P \lor Q$ as a premise,
as the assumption of a subproof, or as something proved before.
We'll try to use it by applying $\lor$Elim.
\end{tabular}

}

\subsec{Strategy for Using Disjunctions}{

\begin{tabular}{@{}l@{}p{13em}}
\fitchprf{
   \pline[1.]{P \lor Q} }{ \subproof{\pline[2.]{P}}{ \ellipsesline \\
\pline[3.]{R}} \subproof{\pline[4.]{Q}}{ \ellipsesline \\
\pline[5.]{R}} \pline[6.]{R}[\lore{1}{2--3}{4--5}] } 
& To prove $\sf R$ using $\lor$Elim from $\sf P \lor Q$, we'll have to
look for two subproofs: one in which we prove $\sf R$ from $\sf P$,
another where we prove $\sf R$ from $\sf Q$. Once we have both, we
can justify $\sf R$ by using $\lor$Elim, citing the line with $\sf P
\lor Q$ and the two subproofs.
\end{tabular}
}

\subsec{Strategy for Proving Negations}{

\begin{tabular}{@{}lp{13em}}
\fitchprf{
   \pline[1.]{}
}{
 \pline{}\\
\pline{} \\
\pline{}\\
\ellipsesline \\[.7em]
  \pline[4.]{\neg P}[\hphantom{\lnoti{2}}]
} 
  &
If we want to prove $\neg\sf P$, we'll have to use  $\neg$Intro.
\end{tabular}

}

\subsec{Strategy for Proving Negations}{

\begin{tabular}{@{}lp{13em}}
\fitchprf{\pline[1.]{}}{
\subproof{\pline[2.]{P}}{
\ellipsesline \\
\pline[3.]{\bot}}
\pline[4.]{\neg P}[\lnoti{2--3}]
} 
& For $\neg$Intro, we have to start a subproof with assumption $\sf
P$; the last line of the subproof has to be $\bot$.  We'll cite the
subproof, and use $\lnot$Intro.
\end{tabular}
}


\subsec{Strategy for Indirect Proof}{

\begin{tabular}{@{}lp{13em}}
\fitchprf{
   \pline[1.]{}
}{
 \pline{}\\
\pline{} \\
\pline{}\\
\ellipsesline \\[.7em]
  \pline[4.]{P}[\hphantom{\lnoti{2}}]
} 
& Sometimes, we want to prove a sentence $\sf P$, but our other
strategies didn't get us far. This is often the case, e.g., when we
want to prove disjunctions but don't have any premises (for example:
$\sf A \lor \neg A$).  Then we can also use $\neg$Intro.
\end{tabular}

}

\subsec{Strategy for Indirect Proof}{

\begin{tabular}{@{}lp{13em}}
\fitchprf{\pline[1.]{}}{
\subproof{\pline[2.]{\neg P}}{
\ellipsesline \\
\pline[3.]{\bot}}
\pline[4.]{P}[\lnoti{2--3}]} 
&
Here, we have to start a subproof with assumption $\sf \neg P$;
the last line of the subproof has to be $\bot$.
We'll cite the subproof, and use $\lnot$Intro.  In the subproof, we now
have an additional assumption (on line 2) to work with.
\end{tabular}

}

\subsec{How to Find a Contradiction}{

\begin{tabular}{@{}lp{13em}}
\fitchprf{\pline[1.]{}}{
\subproof{\pline[2.]{\neg P}}{
\pline{}\\
\ellipsesline \\
\pline[4.]{\bot}}
\pline[5.]{P}[\lnoti{2--3}]
} 
&
Suppose we used the indirect proof strategy, or we're in some other situation
where we're looking for a proof of $\bot$.  What's a good candidate?
\end{tabular}

}

\subsec{How to Find a Contradiction}{

\begin{tabular}{@{}lp{13em}}
\fitchprf{\pline[1.]{}}{
\subproof{\pline[2.]{\neg P}}{
\ellipsesline \\
\pline[3.]{P}\\
\pline[4.]{\bot}[\lfalsei{2}{3}]}
\pline[5.]{P}[\lnoti{2--4}]
} 
& One good candidate is $\sf P$ itself!  This may look weird but
remember that inside the subproof, we have an additional assumption
$\sf \lnot P$ to work with.
\end{tabular}

}

\subsec{How to Use a Negated Sentence}{

\begin{tabular}{@{}lp{13em}}
\fitchprf{
   \pline[1.]{\neg P}
}{
 \pline{}\\
\pline{} \\
\pline{}\\
\ellipsesline \\[.7em]
  \pline[4.]{R}[\hphantom{\lnoti{2}}]
} 
  &
Suppose $\sf\neg P$ is one of your premises, or something else you've
already proved, and the sentence you're shooting for doesn't contain
$\sf \neg P$. How are you going to make use of  $\sf\neg P$?
\end{tabular}

}

\subsec{How to Use a Negated Sentence}{

\begin{tabular}{@{}lp{13em}}
\fitchprf{\pline[1.]{\neg P}}{
\subproof{\pline[2.]{\neg R}}{
\ellipsesline \\
\pline[3.]{P}\\
\pline[4.]{\bot}[\lfalsei{1}{3}]}
\pline[5.]{R}[\lnoti{2--4}]
} 
&
The only way to make use of $\sf\neg P$ in such a situation is as part
of a contradiction. For instance, apply the indirect proof strategy,
and then look for $\sf P$ inside the subproof.
\end{tabular}

}

\subsec{Summary}{

\bits
\item Trying to prove $\sf P \land Q$? Look for a proof of $\sf P$,
  then for a proof of $\sf Q$ ($\land$Intro).
\item Split up conjunctions ($\land$Elim) whenever you can.
\item Next, use the disjunctions you have ($\lor$Elim).
\item Trying to prove $\sf\neg P$? Look for a subproof of $\bot$ from
  $\sf P$ ($\neg$Intro).
\item Trying to prove $\sf P \lor Q$?  Look for a proof of $\sf P$, if
  that doesn't work, look for a proof of $\sf Q$ ($\lor$Intro). If
  that doesn't work either, use indirect proof.  (Note: $\lor$Intro
  rarely works unless you're in a subproof.)
\item Apply the strategies at each step in the construction of your
  proof. You may not be able to prove $\sf P \lor Q$ using $\lor$Intro
  at one point, but then you might find yourself in a subproof where
  it is possible.
\eit
}

\subsec{Summary}{
\bits
\item It's good to know where you're going: So use the strategies
  based on $\land$Intro, $\lor$Elim, $\neg$Intro before those based on
  $\land$Elim and $\lor$Intro.
\item Picking a disjunct to prove for $\lor$Intro or a candidate for a
  contradiction doesn't always work. If it doesn't, you have to
  backtrack and try something else.
\item If you're looking for a proof of $\sf P$ and you're not getting
  anywhere, make sure you're on the right track: is $\sf P$ even a
  tautological consequence of the premises and assumptions? If not,
  you'll have to backtrack.
\end{itemize}

}

\section{Examples}

\setlength{\fitchprfwidth}{1.4in}

\subsec{An Example}{

\begin{tabular}{@{}p{13em}@{}p{13em}}
\fitchprf{
   \pline[1.]{(A \land B) \lor (A \land C)}
}{
 \pline{}\\
\pline{} \\
\pline{}\\
\ellipsesline \\[.7em]
  \pline{A \land (B \lor C)}[\hphantom{\lore{1}{2--5}{6--9}}]
} 
  &
First, we use the disjunction on line 1, and set up the subproofs we
need for $\lor$Elim.
\end{tabular}

}
\subsec{An Example}{

\begin{tabular}{@{}p{13em}@{}p{13em}}
\fitchprf{
   \pline[1.]{(A \land B) \lor (A \land C)}
}{
\subproof{\pline[2.]{A \land B}}{
\ellipsesline \\
  \pline[6.]{A \land (B \lor C)}}\\[.5ex]
\subproof{\pline[7.]{A \land C}}{
\ellipsesline \\
  \pline[11.]{A \land (B \lor C)}}
  \pline{A \land (B \lor C)}[\lore{1}{2--6}{7--11}]
} 
  &
In the first subproof, we now set up the sub goals for proving line 6
using $\land$Intro.
\end{tabular}

}
\subsec{An Example}{

\begin{tabular}{@{}p{13em}@{}p{13em}}
\fitchprf{
   \pline[1.]{(A \land B) \lor (A \land C)}
}{
\subproof{\pline[2.]{A \land B}}{
\ellipsesline \\
  \pline[4.]{A}\\
  \pline[5.]{B \lor C}\\
  \pline[6.]{A \land (B \lor C)}[\landi{4, 5}]}\\[.5ex]
\subproof{\pline[7.]{A \land C}}{
  \ellipsesline \\
  \pline[11.]{A \land (B \lor C)}}
\pline{A \land (B \lor C)}[\lore{1}{2--6}{7--11}]
} 
  &
We immediately see that we get line 4 from 2 by $\land$Elim; let's
apply the strategy for proving disjunctions to line 5: look for a
proof of $\sf B$.
\end{tabular}


}
\subsec{An Example}{

\begin{tabular}{@{}p{13em}@{}p{13em}}
\fitchprf{
   \pline[1.]{(A \land B) \lor (A \land C)}
}{
\subproof{\pline[2.]{A \land B}}{
  \pline[3.]{B}\\
  \pline[4.]{A}[\lande{2}]\\
  \pline[5.]{B \lor C}[\lori{3}]\\
  \pline[6.]{A \land (B \lor C)}[\landi{4, 5}]}\\[.5ex]
\subproof{\pline[7.]{A \land C}}{
\ellipsesline \\
  \pline[11.]{A \land (B \lor C)}}
  \pline[12.]{A \land (B \lor C)}[\lore{1}{2--6}{7--11}]
} 
  &
Like line 4 before, we get line 3 from 2 by $\land$Elim. That's it for
the first subproof. The second subproof is exactly the same.
\end{tabular}

}
\subsec{An Example}{

\begin{tabular}{@{}p{13em}@{}p{13em}}
\fitchprf{
   \pline[1.]{(A \land B) \lor (A \land C)}
}{
\subproof{\pline[2.]{A \land B}}{
  \pline[3.]{B}[\lande{2}]\\
  \pline[4.]{A}[\lande{2}]\\
  \pline[5.]{B \lor C}[\lori{3}]\\
  \pline[6.]{A \land (B \lor C)}[\landi{4, 5}]}\\[.5ex]
\subproof{\pline[7.]{A \land C}}{
  \pline[8.]{C}[\lande{7}]\\
  \pline[9.]{A}[\lande{7}]\\
  \pline[10.]{B \lor C}[\lori{8}]\\
  \pline[11.]{A \land (B \lor C)}[\landi{9, 10}]}
  \pline[12.]{A \land (B \lor C)}[\lore{1}{2--6}{7--11}]
} 
  &
\end{tabular}

}

\setlength{\fitchprfwidth}{1.2in}

\subsec{Example Indirect Proof}{

\begin{tabular}{@{}p{14em}@{}p{12em}}
\fitchprf{\pline[1.]{}}{
\subproof{\pline[2.]{\neg (P \lor \lnot P)}}{
\ellipsesline\\
\pline[8.]{\bot}[\lfalsei{2}{7}]}
\pline[9.]{P \lor \neg P}[\lnoti{2--8}]
} 
&
Suppose we want to prove $\sf P \lor \neg P$.  A little reflection
shows that this can only be done by indirect proof.  So we set up a subproof
for use with $\neg$Intro.
\end{tabular}

}

\subsec{Example Indirect Proof}{

\begin{tabular}{@{}p{14em}p{12em}}
\fitchprf{\pline[1.]{}}{
\subproof{\pline[2.]{\neg (P \lor \lnot P)}}{
\ellipsesline\\
\pline[7.]{P \lor \neg P}[?]\\
\pline[8.]{\bot}[\lfalsei{2}{7}]}
\pline[9.]{P \lor \neg P}[\lnoti{2--8}]
} 
&
Our first candidate for a contradiction is the assumption of the
subproof.  How should we get $\sf P \lor \neg P$ inside that
subproof?
\end{tabular}

}
\subsec{Example Indirect Proof}{

\begin{tabular}{@{}p{14em}p{12em}}
\fitchprf{\pline[1.]{}}{
\subproof{\pline[2.]{\neg (P \lor \lnot P)}}{
\subproof{\pline[3.]{P}}{
\ellipsesline\\
\pline[5.]{\bot}[?]
}
\pline[6.]{\neg P}[\lnoti{3--5}]\\
\pline[7.]{P \lor \neg P}[\lori{6}]\\
\pline[8.]{\bot}[\lfalsei{2}{7}]}
\pline[9.]{P \lor \neg P}[\lnoti{2--8}]
} 
&
Inside the subproof, we \emph{can} get $\sf P \lor \neg P$ by
$\lor$Intro. So let's try to prove $\sf \neg P$; it's a negated
sentence, so we'll use $\neg$Intro.
\end{tabular}

}
\subsec{Example Indirect Proof}{

\begin{tabular}{@{}p{14em}p{12em}}
\fitchprf{\pline[1.]{}}{
\subproof{\pline[2.]{\neg (P \lor \lnot P)}}{
\subproof{\pline[3.]{P}}{
\pline[4.]{P \lor \neg P}[\lori{3}]\\
\pline[5.]{\bot}[\lfalsei{2}{4}]
}
\pline[6.]{\neg P}[\lnoti{3--5}]\\
\pline[7.]{P \lor \neg P}[\lori{6}]\\
\pline[8.]{\bot}[\lfalsei{2}{7}]}
\pline[9.]{P \lor \neg P}[\lnoti{2--8}]
} 
&
Here, the assumption of the subproof, $\sf P$, is not
really a good candidate for a negation. But we can use the negated
sentence on line 2 again, and it's easy to get in this situation.
\end{tabular}

}


\section{A Logic Puzzle}

\subsec{A Logic Puzzle}{

\bit
\item Every card has a letter on one side and a number on the other side
\item You're a card inspector tasked with making sure that cards satisfy this quality standard:
\begin{quote}
If a card has an even number on one side, then it has a vowel on the other. 
\end{quote}
\eit

}

\subsec{A Logic Puzzle}{

Which card(s) do you have to turn over to make sure that:
\begin{quote}
If a card has an even number on one side, then it has a vowel on the other. 
\end{quote}

\begin{tabular}{cccc}
\begin{beamerboxesrounded}[width=4em]{}
\vskip 2ex
\hfil \Large E\hfil\\
\end{beamerboxesrounded} &
\begin{beamerboxesrounded}[width=4em]{}
\vskip 2ex
\hfil \Large K\hfil\\
\end{beamerboxesrounded} &
\begin{beamerboxesrounded}[width=4em]{}
\vskip 2ex
\hfil \Large 3\hfil\\
\end{beamerboxesrounded} &
\begin{beamerboxesrounded}[width=4em]{}
\vskip 2ex
\hfil \Large 4\hfil\\
\end{beamerboxesrounded} \\
(1) & (2) & (3) & (4)
\end{tabular}

}

\subsec{Another Logic Puzzle}{

\bit
\item At an all-ages event where everyone has a drink
\item You know how old some of the people are, and you can tell what some of them are drinking
\item You're tasked with making sure that the following rule is followed:
\begin{quote}
If a person is drinking alcohol, then they must be at least 18 years old.
\end{quote}
\eit

}
\subsec{Another Logic Puzzle}{

Which of these people do you have to check (age or drink) to ensure that:
\begin{quote}
If a person is drinking alcohol, then they must be at least 18 years old
\end{quote}

\begin{tabular}{cccc}
\begin{beamerboxesrounded}[width=4em]{}
\vskip 2ex
\Large 22 years\\
\end{beamerboxesrounded} &
\begin{beamerboxesrounded}[width=4em]{}
\vskip 2ex
\Large 16 years\\
\end{beamerboxesrounded} &
\begin{beamerboxesrounded}[width=4em]{}
\vskip 2ex
\Large drinks pop\\
\end{beamerboxesrounded} &
\begin{beamerboxesrounded}[width=4em]{}
\vskip 2ex
\Large drinks beer\\
\end{beamerboxesrounded} \\
(1) & (2) & (3) & (4)
\end{tabular}

}



\end{document}




